NFA.thy
@@ -17,7 +17,6 @@ record ('q,'a) NFA_rec =
   \<Q> :: "'q set"           (* "The set of states" *)
   \<Sigma> :: "'a set"           (* alphabet *)
   \<Delta> :: "('q,'a) LTS"      (* "The transition relation" *)
-  \<Delta>' :: "('q*'q) set"      (* "The transition relation" *)
   \<I> :: "'q set"            (* "The set of initial states *)
   \<F> :: "'q set"           (* "The set of final states *)
 
@@ -25,10 +24,8 @@ text \<open>Using notions for labelled transition systems,
 it is easy to define the languages accepted by automata.\<close>
 
 definition NFA_accept :: "('a, 'b) NFA_rec \<Rightarrow> 'b list \<Rightarrow> bool" where
-  "NFA_accept \<A> w = (if \<Delta>' \<A> \<noteq> {} then
-                  (\<exists> q \<in> (\<I> \<A>). \<exists> q' \<in> (\<F> \<A>). \<exists> (q,q'') \<in> (\<Delta>' \<A>).LTS_is_reachable (\<Delta> \<A>) q'' w q')  
-                        else (\<exists> q \<in> (\<I> \<A>). \<exists> q' \<in> (\<F> \<A>).
-                  LTS_is_reachable (\<Delta> \<A>) q w q')) "
+  "NFA_accept \<A> w = (\<exists> q \<in> (\<I> \<A>). \<exists> q' \<in> (\<F> \<A>).
+                  LTS_is_reachable (\<Delta> \<A>) q w q') "
 
 definition \<L> where "\<L> \<A> = {w. NFA_accept \<A> w}"
 
